proofs/transform/eliminate_algebraic_proofs/eliminate_algebraic_typing.v
@@ -72,6 +72,275 @@ Proof.
   clear Hty.
   unfold fold_all_ctx_gamma. *)
 
+(*Signature of new gamma (and prove NoDups)*)
+
+(*TODO: better for induction, move*)
+
+Lemma sig_f_app (g1 g2: context):
+  sig_f (g1 ++ g2) = sig_f g1 ++ sig_f g2.
+Proof.
+  unfold sig_f; rewrite map_app, concat_app; reflexivity.
+Qed.
+
+Require Import GenElts.
+
+Lemma projection_axioms_syms (c: funsym) l:
+  length l = length (s_args c) ->
+  map fst (projection_axioms new_constr_name badnames c l) = l.
+Proof.
+  intros Hlen.
+  unfold projection_axioms.
+  rewrite map_snd_combine; [| rewrite gen_names_length; auto].
+  match goal with
+  |- map ?f (map2 ?g ?l1 ?l2) = _ =>
+    let Hlen := fresh "Hlen2" in
+    assert (Hlen2: length l1 = length l2) by (unfold vsymbol in *; simpl_len;
+      rewrite gen_names_length; lia);
+    generalize dependent l1
+  end. clear Hlen.
+  induction l as [| h1 t1 IH]; intros [| h2 t2]; simpl; auto; try discriminate.
+  intros Hlen. f_equal; auto.
+Qed.
+
+(*TODO: can move projection_syms_length*)
+Require Import eliminate_algebraic_interp.
+
+Lemma mut_in_ctx_cons d gamma m:
+  mut_in_ctx m (d :: gamma) =
+  (match d with
+    | datatype_def m1 => mut_adt_dec m m1
+    | _ => false
+  end) || mut_in_ctx m gamma.
+Proof.
+  destruct d; auto.
+Qed.
+
+(*NOTE: [keep_muts] is annoying: not everything in old gamma is in new gamma
+  Options:
+  1. Only prove 1 direction (but we do want to know things are in)
+    then prove that new stuff is in (but don't say anything about old/only
+    prove old with valid context)
+  2. Just assume valid context*)
+
+(*For now, split into 3 lemmas:
+  1. Prove if in sig_f, the implication holds
+  2. Prove that if we have any of the newly added, it is in the result
+  3. Prove that under valid context, certain subset is in the result*)
+
+Lemma in_sig_f_new_gamma_gen gamma gamma2 f: 
+  In f (sig_f (fold_all_ctx_gamma_gen new_constr_name keep_muts badnames noind gamma gamma2)) ->
+   (*new constrs*)
+  (exists m a c, mut_in_ctx m gamma /\ adt_in_mut a m /\ constr_in_adt c a /\
+    f = new_constr new_constr_name badnames c) \/
+  (*projections*)
+  (exists m a c, mut_in_ctx m gamma /\ adt_in_mut a m /\ constr_in_adt c a /\
+    In f (projection_syms badnames c)) \/
+  (*selector*)
+  (exists m a, mut_in_ctx m gamma /\ adt_in_mut a m /\
+    negb (single (adt_constr_list a)) /\
+    f = selector_funsym badnames  (adt_name a) (adt_constr_list a)) \/
+  (*indexer*)
+  (exists m a, mut_in_ctx m gamma /\ adt_in_mut a m /\
+    negb (single (adt_constr_list a)) && negb (noind (adt_name a)) /\
+    f = indexer_funsym badnames (adt_name a)) \/
+  (*in gamma*)
+  In f (sig_f gamma).
+Proof.
+  unfold fold_all_ctx_gamma_gen.
+  induction gamma as [| d gamma IH]; auto.
+  simpl sig_f.
+  rewrite sig_f_app. rewrite in_app_iff.
+  intros [Hinnew | Hinold].
+  - (*In new*)
+    setoid_rewrite mut_in_ctx_cons. simpl. unfold comp_ctx_gamma in Hinnew. destruct d; simpl in *;
+    try contradiction; (*really bad*)
+    try (unfold sig_f in Hinnew; simpl in Hinnew; rewrite app_nil_r in Hinnew;
+      try unfold TaskGen.funpred_def_map in Hinnew; simpl in Hinnew;
+      try destruct f0; simpl in Hinnew; destruct_all; subst; try contradiction;
+      unfold sig_f; simpl; try rewrite in_app_iff;
+      repeat(right; auto) (*TODO: why doesnt destruct_all work here? ught*)).
+    2: destruct_all; subst; repeat(right; auto); try contradiction.
+    (*Now deal with main case*)
+    rewrite sig_f_app in Hinnew.
+    rewrite in_app_iff in Hinnew.
+    destruct Hinnew as [Hin | Hin].
+    -- (*New axiom funsyms added*)
+      unfold sig_f in Hin. rewrite concat_map, !map_map in Hin.
+      rewrite in_concat in Hin. destruct Hin as [l1 [Hinl1 Hinf]].
+      rewrite in_concat in Hinl1. destruct Hinl1 as [l2 [Hinl2 Hinl1]].
+      rewrite in_map_iff in Hinl2. destruct Hinl2 as [a [Hl2 Hina]].
+      rewrite <- In_rev in Hina.
+      subst. rewrite in_map_iff in Hinl1.
+      destruct Hinl1 as [d [Hl1 Hind]].
+      subst. unfold add_axioms_gamma in Hind.
+      rewrite !in_app_iff in Hind.
+      assert (m_in: mut_in_ctx m (datatype_def m :: gamma)). {
+        unfold mut_in_ctx. simpl. destruct (mut_adt_dec m m); auto.
+      }
+      assert (a_in: adt_in_mut a m). {
+        apply In_in_bool; auto.
+      }
+      destruct Hind as [Hind | [Hind | [Hind | Hind]]].
+      ++ (*projection*)
+        right. left. rewrite concat_map, !map_map in Hind.
+        rewrite in_concat in Hind. destruct Hind as [ds [Hinds Hind]].
+        rewrite in_map_iff in Hinds. destruct Hinds as [c [Hds Hinc]]; subst.
+        rewrite <- In_rev in Hinc.
+        rewrite map_rev, map_map, <- In_rev in Hind.
+        rewrite in_map_iff in Hind. destruct Hind as [[f1 nf] [Hd Hinf1]];
+        simpl in Hd; subst. simpl in Hinf. destruct Hinf as [Heq | []]; subst.
+        apply (in_map fst) in Hinf1.
+        simpl in Hinf1.
+        rewrite projection_axioms_syms in Hinf1 by
+          (rewrite projection_syms_length; lia).
+        exists m. exists a. exists c. split_all; auto.
+        apply constr_in_adt_eq; auto.
+      ++ (*indexer*)
+        destruct (_ && _) eqn : Hb; simpl in Hind;
+        [destruct Hind as [Hd | []] | destruct Hind].
+        subst. simpl in Hinf. destruct Hinf as [Heq | []]; subst.
+        right; right; right; left. exists m; exists a; auto.
+      ++ (*selector*)
+        destruct (negb _) eqn : Hb; simpl in Hind; destruct_all; subst; try contradiction.
+        simpl in Hinf. destruct Hinf as [Heq | []]; subst.
+        right; right; left. exists m; exists a; auto.
+      ++ (*new constr*)
+        rewrite <- In_rev, !map_map in Hind.
+        rewrite in_map_iff in Hind. destruct Hind as [c [Hd Hc]]; subst.
+        simpl in Hinf. destruct Hinf as [Heq | []]; subst.
+        left. exists m; exists a; exists c; split_all; auto.
+        apply constr_in_adt_eq; auto.
+    -- (*In this case, existing constr or not funsym*)
+      destruct (keep_muts m); simpl in Hin.
+      ++ unfold sig_f in Hin; simpl in Hin.
+        rewrite app_nil_r in Hin.
+        repeat right. unfold sig_f; simpl.
+        rewrite in_app_iff; auto.
+      ++ exfalso. clear -Hin.
+        (*Could do separate lemma?*)
+        rewrite <- map_rev in Hin.
+        induction (rev (typs m)) as [| h t IH]; simpl in Hin; auto.
+  - (*In rest*)
+    apply IH in Hinold; clear IH.
+    assert (Hmimpl: forall m, mut_in_ctx m gamma -> mut_in_ctx m (d :: gamma)).
+    { intros m. rewrite mut_in_ctx_cons. intros Hm; rewrite Hm, orb_true_r. auto. } 
+    destruct_all; subst; eauto 11.
+    repeat right. unfold sig_f in *; simpl; rewrite in_app_iff; auto 10.
+Qed.
+
+Lemma prove_or_impl_r (P Q R: Prop):
+  (P -> Q) ->
+  (R \/ P) ->
+  (R \/ Q).
+Proof. tauto. Qed.
+
+Lemma new_in_sig_f_new_gamma_gen gamma gamma2 f: 
+   (*new constrs*)
+  (exists m a c, mut_in_ctx m gamma /\ adt_in_mut a m /\ constr_in_adt c a /\
+    f = new_constr new_constr_name badnames c) \/
+  (*projections*)
+  (exists m a c, mut_in_ctx m gamma /\ adt_in_mut a m /\ constr_in_adt c a /\
+    In f (projection_syms badnames c)) \/
+  (*selector*)
+  (exists m a, mut_in_ctx m gamma /\ adt_in_mut a m /\
+    negb (single (adt_constr_list a)) /\
+    f = selector_funsym badnames  (adt_name a) (adt_constr_list a)) \/
+  (*indexer*)
+  (exists m a, mut_in_ctx m gamma /\ adt_in_mut a m /\
+    negb (single (adt_constr_list a)) && negb (noind (adt_name a)) /\
+    f = indexer_funsym badnames (adt_name a)) ->
+  In f (sig_f (fold_all_ctx_gamma_gen new_constr_name keep_muts badnames noind gamma gamma2)).
+Proof.
+  unfold fold_all_ctx_gamma_gen.
+  induction gamma as [| d gamma IH]; simpl; auto.
+  - unfold mut_in_ctx. simpl. intros; destruct_all; discriminate.
+  - rewrite sig_f_app. rewrite in_app_iff. setoid_rewrite mut_in_ctx_cons.
+    intros Hcases.
+    apply (prove_or_impl_r _ _ _ IH); clear IH.
+    (*First, handle non-mut*)
+    destruct d.
+    2: {
+      simpl in *; destruct_all; eauto 11;
+      unfold sig_f in *; simpl in *;
+      rewrite in_app_iff in *; destruct_all; auto 6.
+    }
+    all: try solve [simpl in *; destruct_all; [eauto 9 | eauto 10 | eauto 10 | eauto 11 ]].
+    (* 3: {
+      (*need explicit levels or else takes LONG time*)
+      simpl in *; destruct_all; [eauto 9 | eauto 10 | eauto 10 | eauto 11 | eauto 3 | eauto 6].
+    }
+    2: {
+      destruct f0; simpl in *; destruct_all; 
+        [eauto 9 | eauto 10 | eauto 10 | eauto 11 | eauto 6 | eauto 6 | eauto 9 |
+          eauto 10 | eauto 10 | eauto 11 | eauto 6 ].
+    } *)
+    (*datatype def is interesting case*)
+    (*Simplify comp_ctx once*)
+    unfold sig_f at 1. unfold comp_ctx_gamma.
+    rewrite map_app, concat_app, in_app_iff,
+    !concat_map, !map_map, !in_concat.
+    setoid_rewrite in_concat.
+    setoid_rewrite in_map_iff.
+    setoid_rewrite <- In_rev.
+    (*Now cases*)
+    destruct Hcases as [[m1 [a [c [m_in [a_in [c_in Hf]]]]]]| 
+      [[m1 [a [c [m_in [a_in [c_in Hinf]]]]]] | 
+      [[m1 [a [m_in [a_in [Hconstr Hf]]]]] | 
+      [m1 [a [m_in [a_in [Hconstr Hf]]]]]]]].
+    * (*new constr*)
+      destruct (mut_adt_dec m1 m); subst; simpl in m_in; [|eauto 10].
+      left. left. exists ([(new_constr new_constr_name badnames c)]); split; [|simpl; auto].
+        (*(map (new_constr new_constr_name badnames) (adt_constr_list a)).*)
+      (* split; [| apply in_map; auto; apply constr_in_adt_eq; auto]. *)
+      eexists. split; [exists a; split; [reflexivity|] |].
+      -- apply in_bool_In in a_in. auto.
+      -- unfold add_axioms_gamma. rewrite !map_app.
+        rewrite !in_app_iff.
+        right. right. right. rewrite map_rev, <- In_rev, !map_map. simpl.
+        rewrite in_map_iff. exists c; split; auto. apply constr_in_adt_eq; auto.
+    * (*projection*)
+      destruct (mut_adt_dec m1 m); subst; simpl in m_in; [|eauto 10].
+      left. left. exists [f]; split; auto. (*exists (projection_syms badnames c).*)
+      eexists. split; [exists a; split; [reflexivity|]|].
+      -- apply in_bool_In in a_in. auto.
+      -- unfold add_axioms_gamma. rewrite !map_app.
+        rewrite !in_app_iff. left.
+        rewrite map_map. simpl.
+        rewrite in_map_iff. exists f; split; auto.
+        rewrite in_concat. exists (rev (projection_syms badnames c)).
+        rewrite <- In_rev. split; auto.
+        rewrite in_map_iff. exists c. rewrite <- In_rev. split; auto;
+        [|apply constr_in_adt_eq; auto].
+        f_equal. apply projection_axioms_syms. apply projection_syms_length.
+      -- simpl; auto.
+    * (*selector*)
+      subst. destruct (mut_adt_dec m1 m); subst; simpl in m_in; [|eauto 10].
+      left. left. exists [selector_funsym badnames (adt_name a) (adt_constr_list a)]; split;
+      [| simpl; auto].
+      eexists. split; [exists a; split; [reflexivity|] |].
+      -- apply in_bool_In in a_in. auto.
+      -- unfold add_axioms_gamma. rewrite !map_app.
+        rewrite !in_app_iff. right. right. left.
+        destruct (negb (single (adt_constr_list a))); simpl; auto.
+    * (*indexer*)
+      subst. destruct (mut_adt_dec m1 m); subst; simpl in m_in; [|solve[eauto 11]].
+      left. left. exists [indexer_funsym badnames (adt_name a)]; split;
+      [| simpl; auto].
+      eexists. split; [exists a; split; [reflexivity|] |].
+      -- apply in_bool_In in a_in. auto.
+      -- unfold add_axioms_gamma. rewrite !map_app.
+        rewrite !in_app_iff. right. left. rewrite Hconstr. simpl. auto.
+Qed.
+
+(*TODO: later, prove that if context is valid, then everything in old
+  signature EXCEPT for constructors for ADTs such that [keep_muts] is false,
+  is in new sig_f - need valid to show that these symbols dont intersect with
+  anything else*)
+
+
+(*TODO: going to need valid_context to show that f_is_constr imples f constructo*)
+
+
 Lemma tfun_ty_change_sym gamma (f1 f2: funsym) tys tms ty:
   s_args f1 = s_args f2 ->
   s_params f1 = s_params f2 ->
